theories/iris/examples/effects/coroutines.v
@@ -193,7 +193,7 @@ Section yield_par.
       iSimpl.
       iFrame.
       iSplit; first done.
-      iIntros "HI".
+      iIntros "!> HI".
       iIntros (LI HLI).
       move/lfilledP in HLI.
       inversion HLI; subst.
@@ -201,7 +201,8 @@ Section yield_par.
       iSimpl.
       iApply (ewp_label_value with "[HI]").
       done.
-      by instantiate (1 := λ v f, (⌜ v = immV _ ⌝ ∗ ⌜ f = Build_frame _ _ ⌝ ∗ I)%I); iFrame.
+(*      auto_instantiate. *)
+      by instantiate (1 := λ v f, (⌜ v = immV _ ⌝ ∗ ⌜ f = Build_frame _ _ ⌝ ∗ I)%I); iFrame. 
 
       2: by iIntros (?) "[% _]".
       iIntros (??) "(-> & -> & HI)".
@@ -337,13 +338,13 @@ Section yield_par.
       instantiate (2 := λ f, True%I).
       instantiate (1 := λ v, (⌜ v = immV [] ⌝ ∗ Q1 v ∗ Q2 v ∗ I)%I). *)
       
-      iAssert ( ∀ kaddra kaddrb b tfa conta,
-                  (I ∗ N.of_nat kaddra ↦[wcont] Cont_hh tfa conta  ∗
-                     (I -∗ ∃ LI, ⌜ hfilled No_var conta [] LI ⌝ ∗ EWP LI UNDER empty_frame <| Ψ |> {{ v ; f , ⌜ v = immV [] ⌝ ∗ Q1 ∗ I }})  ∗
-                     ((⌜ b = 0 ⌝ ∗ ∃ tfb contb, N.of_nat kaddrb ↦[wcont] Cont_hh tfb contb ∗ (I -∗ ∃ LI, ⌜ hfilled No_var contb [] LI ⌝ ∗ EWP LI UNDER empty_frame <| Ψ |> {{ v ; f , ⌜ v = immV [] ⌝ ∗ Q2 ∗ I }})) ∨ (⌜ b = 1 ⌝ ∗ Q2))) ∨
-                    (N.of_nat kaddra ↦[wcont] Cont_hh tfa conta  ∗
-                       (I -∗ ∃ LI, ⌜ hfilled No_var conta [] LI ⌝ ∗ EWP LI UNDER empty_frame <| Ψ |> {{ v ; f , ⌜ v = immV [] ⌝ ∗ Q2 ∗ I }})  ∗
-                       ((⌜ b = 0 ⌝ ∗ ∃ tfb contb, N.of_nat kaddrb ↦[wcont] Cont_hh tfb contb ∗ (I -∗ ∃ LI, ⌜ hfilled No_var contb [] LI ⌝ ∗ EWP LI UNDER empty_frame <| Ψ |> {{ v ; f , ⌜ v = immV [] ⌝ ∗ Q1 ∗ I }})) ∨ (⌜ b = 1 ⌝ ∗ Q1)))  -∗
+      iAssert ( ∀ kaddra kaddrb b conta,
+                  (I ∗ N.of_nat kaddra ↦[wcont] Cont_hh emptyt conta  ∗
+                     (I -∗ ∃ LI, ⌜ hfilled No_var conta [] LI ⌝ ∗ ▷ EWP LI UNDER empty_frame <| Ψ |> {{ v ; f , ⌜ v = immV [] ⌝ ∗ Q1 ∗ I }})  ∗
+                     ((⌜ b = 0 ⌝ ∗ ∃ contb, N.of_nat kaddrb ↦[wcont] Cont_hh emptyt contb ∗ (I -∗ ∃ LI, ⌜ hfilled No_var contb [] LI ⌝ ∗ ▷ EWP LI UNDER empty_frame <| Ψ |> {{ v ; f , ⌜ v = immV [] ⌝ ∗ Q2 ∗ I }})) ∨ (⌜ b = 1 ⌝ ∗ Q2))) ∨
+                    (I ∗ N.of_nat kaddra ↦[wcont] Cont_hh emptyt conta  ∗
+                       (I -∗ ∃ LI, ⌜ hfilled No_var conta [] LI ⌝ ∗ ▷ EWP LI UNDER empty_frame <| Ψ |> {{ v ; f , ⌜ v = immV [] ⌝ ∗ Q2 ∗ I }})  ∗
+                       ((⌜ b = 0 ⌝ ∗ ∃ contb, N.of_nat kaddrb ↦[wcont] Cont_hh emptyt contb ∗ (I -∗ ∃ LI, ⌜ hfilled No_var contb [] LI ⌝ ∗ ▷ EWP LI UNDER empty_frame <| Ψ |> {{ v ; f , ⌜ v = immV [] ⌝ ∗ Q1 ∗ I }})) ∨ (⌜ b = 1 ⌝ ∗ Q1)))  -∗
                                                                                                                                                                                                                                               EWP [] ++
                                                                                                                                                                                                                                               [AI_basic
                                                                                                                                                                                                                                                  (BI_loop (Tf [] [])
@@ -381,7 +382,7 @@ Section yield_par.
           rewrite /hfilled /hfill //=.
           iApply ("Hspec2" with "HP2 HI"). }
       iLöb as "IH".
-      iIntros (kaddra kaddrb b tfa conta) "H".
+      iIntros (kaddra kaddrb b conta) "H".
       iDestruct "H" as "[H | H]".
       + (* Case where $current is the $f1 function *)
 
@@ -444,16 +445,15 @@ Section yield_par.
         by iIntros (?) "[% ?]".
         iSplitR; last first.
         iFrame "Htag".
-        iSplitR; first done.
         iSplitR.
-        iIntros (w) "(-> & HQ & HI)".
+        iIntros "!>" (w) "(-> & HQ & HI)".
         iApply (ewp_prompt_value with "[-]").
         rewrite to_of_val => //.
         instantiate (1 := λ v, ((⌜ v = immV [] ⌝ ∗ I ∗ Q1) ∨ _)%I).
         iLeft. iFrame. done. 
         iSimpl.
         iSplitL; last done.
-        iIntros (vs kaddr tf h) "Hcont HΨ".
+        iIntros "!>" (vs kaddr h) "Hcont HΨ".
         iApply ewp_value.
         unfold IntoVal.
         apply of_to_val.
@@ -469,15 +469,14 @@ Section yield_par.
         done.
 
         iRight.
-        instantiate (1 := (∃ kaddr vs tf h, ⌜ v = brV _ ⌝ ∗ _)%I). (* may need a disjunct later *) 
-        iExists kaddr, vs, tf, h. iSplit; first done.
+        instantiate (1 := (∃ kaddr vs h, ⌜ v = brV _ ⌝ ∗ _)%I). 
+        iExists kaddr, vs, h. iSplit; first done.
         iCombine "Hcont HΨ" as "H".
         iExact "H".
-        (*        by iIntros (?) "H". *)
-        iIntros "[[% _] | (% & % & % & % & % & _)]" => //.
+        iIntros "[[% _] | (% & % & % & % & _)]" => //.
         
         iIntros (??) "[H ->]".
-        iDestruct "H" as "[(-> & HI & HQ) | (%kaddr & %vs & %tf & %h & -> & Hcont & HΨ)]".
+        iDestruct "H" as "[(-> & HI & HQ) | (%kaddr & %vs & %h & -> & Hcont & HΨ)]".
         * (* Case 1: the continuation terminated execution *)
           iSimpl.
           rewrite (separate1 (AI_basic (BI_get_local _))).
@@ -559,10 +558,7 @@ Section yield_par.
                                                                                                                                                  (VH_base 1 []
                                                                                                                                                     [AI_basic (BI_const (xx 1)); AI_basic (BI_set_local 4);
                                                                                                                                                      AI_basic (BI_get_local 3); AI_basic (BI_set_local 2); 
-                                                                                                                                                     AI_basic (BI_br 1)]) []) ⌝ ∗ ⌜ f = Build_frame _ _ ⌝ ∗ _) ∨ (∃ kaddr tf h, ⌜ v = immV _ ⌝ ∗ ⌜ f = Build_frame _ _ ⌝%I ∗ _))%I). (* Add fourth disjunct later? *)
-            (*               instantiate (1 := λ f, (⌜ b = 0 ⌝ ∗ ⌜ f = Build_frame _ _ ⌝ ∨ ⌜ b = 1 ⌝ ∗ ⌜ f = Build_frame _ _ ⌝ ∨ ⌜ f = Build_frame _ _ ⌝)%I). 
-            by iLeft. 
-            instantiate (1 := λ v, ((⌜ b = 0 ⌝ ∗ ∃ contb, ⌜ v = brV _ ⌝ ∗ _) ∨ (⌜ b = 1 ⌝ ∗ ⌜ v = brV _ ⌝ ∗ _) ∨ (∃ kaddr tf h, ⌜ v = immV _ ⌝%I ∗ _) )%I).  *)
+                                                                                                                                                     AI_basic (BI_br 1)]) []) ⌝ ∗ ⌜ f = Build_frame _ _ ⌝ ∗ _) ∨ (∃ kaddr h, ⌜ v = immV _ ⌝ ∗ ⌜ f = Build_frame _ _ ⌝%I ∗ _))%I). 
             iLeft. iExists contb.
             iSimpl.
             iSplit; first done. 
@@ -615,9 +611,6 @@ Section yield_par.
           iApply ewp_value.
           apply of_to_val.
           done.
-          (*          iSplitL; last first.
-          iRight. iRight.
-          iIntros (?) "Hf". *)
           iIntros (LI' HLI').
           move/lfilledP in HLI'; inversion HLI'; subst.
           inversion H8; subst.
@@ -633,15 +626,14 @@ Section yield_par.
           apply of_to_val.
           done.
           iRight. iRight.
-          iNext.
-          iExists kaddr, tf, h.
+          iExists kaddr, h.
           iSplit; first done.
           iSplit; first done.
           iCombine "Hb Hcont HI Hrunb" as "H".
           iExact "H".
-        * iIntros (?) "[[[% _] | (% & % & % & % & % & _)] _]" => //.
+        * iIntros (?) "[[[% _] | (% & % & % & % & _)] _]" => //.
         * iIntros (??) "H".
-          iDestruct "H" as "[(%contb & -> & -> & Hcontb & Hrunb & HI & HQ1) | [(-> & -> & HQ1 & HQ2 & HI) | (%kaddr & %tf & %h & -> & -> & Hb & Hcont & Hrunb)]]".
+          iDestruct "H" as "[(%contb & -> & -> & Hcontb & Hrunb & HI & HQ1) | [(-> & -> & HQ1 & HQ2 & HI) | (%kaddr & %h & -> & -> & Hb & Hcont & HI & Hrunb)]]".
           -- (* Case 1a *)
             iApply ewp_value.
             apply of_to_val.
@@ -658,7 +650,7 @@ Section yield_par.
               rewrite /lfilled /lfill //=. }
             done.
             done.
-            iNext.
+(*            iNext. *)
             iApply ("IH" $! kaddrb kaddrb 1).
             iRight.
             iFrame "Hrunb".
@@ -687,7 +679,7 @@ Section yield_par.
               rewrite /lfilled /lfill //=. }
             done.
             done.
-            iNext.
+(*            iNext. *)
             iApply ewp_value.
             apply of_to_val.
             done.
@@ -802,13 +794,541 @@ Section yield_par.
                   instantiate (1 := LH_base [] _).
                   rewrite /lfilled /lfill //=. }
               done. done.
-              iNext.
+(*              iNext. *)
               iApply "IH".
               iRight.
-              iFrame.
+              iFrame "Hconta Hruna HI".
               iLeft.
+              iSplit; first done.
+              iExists h.
+              iFrame "Hcont".
+              iNext.
+(*              iExact "Hrunb". *)
+              iIntros "HI".
+              iDestruct ("Hrunb" with "HI") as "(%LI' & %HLI' & Hewp)".
+              iExists LI'.
+              iSplit; first by iPureIntro; destruct (hfilled No_var h [] LI').
+              iExact "Hewp".
+            ++ (* Case 2b: the other continuation is also done *)
+              rewrite (separate2 (AI_basic (BI_const _))).
+              iApply ewp_seq.
+              done.
+              iSplitR; last first.
+              iSplitR.
+              iApply ewp_br_if_true.
+              by subst.
+              iApply ewp_value.
+              apply of_to_val.
+              done.
+              iNext.
+              by instantiate (1 := λ v f, (⌜ v = brV _ ⌝ ∗ ⌜ f = Build_frame _ _ ⌝)%I).
+              2: by iIntros (?) "[% _]".
+              iIntros (??) "[-> ->]".
+              iSimpl.
+              iApply ewp_value.
+              apply of_to_val.
+              done.
+              iSimpl.
+              iIntros (LI HLI).
+              move/lfilledP in HLI; inversion HLI; subst.
+              inversion H8; subst.
+              iSimpl.
+              iApply ewp_br.
+              3:{ instantiate (1 := 0).
+                  instantiate (1 := []).
+                  instantiate (1 := LH_base [] _).
+                  rewrite /lfilled /lfill //=. }
+              done. done.
+              iApply "IH".
+              iLeft.
+              iSplitL "HI"; first iExact "HI".
+              instantiate (1 := h).
+              iFrame "Hcont".
+              iSplitL "Hrunb".
+              iIntros "!> HI".
+              iDestruct ("Hrunb" with "HI") as "(%LI' & %HLI' & Hewp)".
+              iExists LI'.
+              iSplit; first by iPureIntro; destruct (hfilled No_var h [] LI').
+              iExact "Hewp".
+              iRight.
+              iFrame. done.
+        * iIntros (?) "H".
+          iDestruct "H" as "[H | H]".
+          iDestruct "H" as (?) "[% _]" => //.
+          iDestruct "H" as "[H | H]".
+          iDestruct "H" as "[% _]" => //.
+          iDestruct "H" as (???) "[% _]" => //.
+      + (* Case where $current is the $f2 function *)
 
-              
+        iApply ewp_loop.
+        done. done. done. done.
+        iNext.
+        iApply (ewp_label_bind with "[-]").
+        2:{ iPureIntro. instantiate (5 := []).
+            rewrite /lfilled /lfill /= app_nil_r //. }
+        rewrite (separate1 (AI_basic (BI_block _ _))).
+        iApply ewp_seq.
+        done.
+        iSplitR; last first.
+        rewrite - (app_nil_l [AI_basic (BI_block _ _)]).
+        iSplitL.
+        iApply ewp_block.
+        done. done. done. done.
+        iNext.
+        iApply (ewp_label_bind with "[-]").
+        2:{ iPureIntro. instantiate (5 := []).
+            rewrite /lfilled /lfill /= app_nil_r //. }
+        rewrite (separate1 (AI_basic (BI_get_local _))).
+        iApply ewp_seq.
+        done.
+        iSplitR; last first.
+        iSplitR.
+        iApply ewp_get_local.
+        done.
+        auto_instantiate.
+        2: by iIntros (?) "[% _]".
+        iIntros (??) "[-> ->]".
+        iSimpl.
+        rewrite (separate2 (AI_ref_cont _)).
+        iApply ewp_seq.
+        done.
+        iSplitR; last first.
+        iDestruct "H" as "(HI & Hconta & Hruna & Hb)".
+        iDestruct ("Hruna" with "HI") as (LI) "[%HLI Hruna]".
+        iSplitR "Hb".
+        rewrite -(app_nil_l [AI_ref_cont _;_]).
+        
+        iApply (ewp_resume with "[$Hconta $Hruna]").
+        done. done. done.
+        simpl. instantiate (1 := [_]) => //.
+        unfold agree_on_uncaptured => /=.
+        repeat split => //.
+        intros i.
+        destruct (i == Mk_tagidx addr_tag) eqn:Hi => //.
+        move/eqP in Hi.
+        intros _.
+        subst Ψ; simpl.
+        destruct i => //.
+        destruct (n =? addr_tag) eqn:Hn => //.
+        apply Nat.eqb_eq in Hn as ->.
+        exfalso; by apply Hi.
+        by subst Ψ.
+        by subst Ψ.
+        by destruct (hfilled No_var conta [] LI).
+        iSplitR.
+        by iIntros (?) "[% ?]".
+        iSplitR; last first.
+        iFrame "Htag".
+        iSplitR.
+        iIntros "!>" (w) "(-> & HQ & HI)".
+        iApply (ewp_prompt_value with "[-]").
+        rewrite to_of_val => //.
+        instantiate (1 := λ v, ((⌜ v = immV [] ⌝ ∗ I ∗ Q2) ∨ _)%I).
+        iLeft. iFrame. done. 
+        iSimpl.
+        iSplitL; last done.
+        iIntros "!>" (vs kaddr h) "Hcont HΨ".
+        iApply ewp_value.
+        unfold IntoVal.
+        apply of_to_val.
+        unfold to_val.
+        rewrite map_app merge_app.
+        specialize (@const_list_to_val (v_to_e_list vs)) as (vs' & Htv & Hinj).
+        apply v_to_e_is_const_list.
+        apply v_to_e_inj in Hinj as ->.
+        unfold to_val in Htv.
+        destruct (merge_values _); try by exfalso.
+        inversion Htv; subst.
+        simpl.
+        done.
+
+        iRight.
+        instantiate (1 := (∃ kaddr vs h, ⌜ v = brV _ ⌝ ∗ _)%I). 
+        iExists kaddr, vs, h. iSplit; first done.
+        iCombine "Hcont HΨ" as "H".
+        iExact "H".
+        iIntros "[[% _] | (% & % & % & % & _)]" => //.
+        
+        iIntros (??) "[H ->]".
+        iDestruct "H" as "[(-> & HI & HQ) | (%kaddr & %vs & %h & -> & Hcont & HΨ)]".
+        * (* Case 1: the continuation terminated execution *)
+          iSimpl.
+          rewrite (separate1 (AI_basic (BI_get_local _))).
+          iApply ewp_seq.
+          done.
+          iSplitR; last first.
+          iSplitR.
+          iApply ewp_get_local.
+          done.
+          auto_instantiate.
+          2: by iIntros (?) "[% _]".
+          iIntros (??) "[-> ->]".
+          iSimpl.
+          iDestruct "Hb" as "[(-> & %contb & Hcont & Hrunb) | (-> & HQ2)]". (* Changed %Hb to -> twice *)
+          -- (* Case 1a: the other continuation is not done *)
+            rewrite (separate2 (AI_basic (BI_const _))).
+            iApply ewp_seq.
+            done.
+            iSplitR; last first.
+            iSplitR.
+            iApply ewp_br_if_false.
+            by subst.
+            auto_instantiate.
+            2: by iIntros (?) "[% _]".
+            iIntros (??) "[-> ->]".
+            iSimpl.
+            rewrite (separate2 (AI_basic (BI_const _))).
+            iApply ewp_seq.
+            done.
+            iSplitR; last first.
+            iSplitR.
+            fold (AI_const (VAL_num (xx 1))).
+            iApply ewp_set_local.
+            simpl; lia.
+            iSimpl.
+            auto_instantiate.
+            2: by iIntros (?) "[% _]".
+            iIntros (??) "[-> ->]".
+            iSimpl.
+            rewrite (separate1 (AI_basic (BI_get_local _))).
+            iApply ewp_seq.
+            done.
+            iSplitR; last first.
+            iSplitR.
+            iApply ewp_get_local.
+            done.
+            auto_instantiate.
+            2: by iIntros (?) "[% _]".
+            iIntros (??) "[-> ->]".
+            iSimpl.
+            rewrite (separate2 (AI_ref_cont _)).
+            iApply ewp_seq.
+            done.
+            iSplitR; last first.
+            iSplitR.
+            fold (AI_const (VAL_ref (VAL_ref_cont kaddrb))).
+            iApply ewp_set_local.
+            simpl; lia.
+            iSimpl.
+            auto_instantiate.
+            2: by iIntros (?) "[% _]".
+            iIntros (??) "[-> ->]".
+            iSimpl.
+            iApply ewp_value.
+            apply of_to_val. done.
+            (*            iSplitL; last first.
+            instantiate (1 := λ f, (⌜ b = 0 ⌝ ∗ ⌜ f = Build_frame _ _ ⌝ ∨ ⌜ b = 1 ⌝ ∗ ⌜ f = Build_frame _ _ ⌝ ∨ ⌜ f = Build_frame _ _ ⌝ )%I).  
+            by iLeft. 
+            iIntros (?) "[[_ ->] | [[% _] | %Hf]]"; try by subst b. *)
+            iIntros (LI' HLI').
+            move/lfilledP in HLI'; inversion HLI'; subst.
+            inversion H8; subst.
+            iSimpl.
+            iApply ewp_value.
+            apply of_to_val.
+            done.
+            iSimpl.
+            instantiate (1 := λ v f, ((∃ contb, ⌜ v = brV (VH_rec [] 1 [] (VH_base 0 [] []) []) ⌝ ∗ ⌜ f = Build_frame _ _ ⌝ ∗ _) ∨ (⌜ v = brV (VH_rec [] 1 []
+                                                                                                                                                 (VH_base 1 []
+                                                                                                                                                    [AI_basic (BI_const (xx 1)); AI_basic (BI_set_local 4);
+                                                                                                                                                     AI_basic (BI_get_local 3); AI_basic (BI_set_local 2); 
+                                                                                                                                                     AI_basic (BI_br 1)]) []) ⌝ ∗ ⌜ f = Build_frame _ _ ⌝ ∗ _) ∨ (∃ kaddr h, ⌜ v = immV _ ⌝ ∗ ⌜ f = Build_frame _ _ ⌝%I ∗ _))%I). 
+            iLeft. iExists contb.
+            iSimpl.
+            iSplit; first done. 
+            iSplit; first done.            
+            iCombine "Hcont Hrunb HI HQ" as "H".
+            iExact "H".
+          -- (* Case 1b: the other continuation is also done *)
+            rewrite (separate2 (AI_basic (BI_const _))).
+            iApply ewp_seq.
+            done.
+            iSplitR; last first.
+            iSplitR.
+            iApply ewp_br_if_true.
+            by subst.
+            iApply ewp_value.
+            apply of_to_val.
+            done.
+            iNext.
+            by instantiate (1 := λ v f, (⌜ v = brV _ ⌝ ∗ ⌜ f = Build_frame _ _ ⌝)%I).
+            2: by iIntros (?) "[% _]".
+            iIntros (??) "[-> ->]".
+            iSimpl.
+            iApply ewp_value.
+            apply of_to_val.
+            done.
+            (*            iSplitL; last first.
+            by iRight.
+            iIntros (?) "[[% _] | [_ ->]]"; first by subst. *)
+            iIntros (LI' HLI').
+            move/lfilledP in HLI'; inversion HLI'; subst.
+            inversion H8; subst.
+            iSimpl.
+            iApply ewp_value.
+            apply of_to_val.
+            done. simpl in *.
+            iRight. iLeft. iSimpl.
+            iSplit; first done.
+            iSplit; first done.
+            iCombine "HQ HQ2 HI" as "H".
+            iExact "H".
+        * (* Case 2: the continuation yielded *)
+          iSimpl.
+          replace (Ψ (SuspendE (Mk_tagidx addr_tag))) with (!immV []{{ I }};? immV [] {{ I }} )%iprot.
+          2:{ subst Ψ. rewrite Nat.eqb_refl. done. }
+          rewrite (upcl_tele' [tele] [tele]).
+          simpl.
+          iDestruct "HΨ" as "(%Heq & HI & Hrunb)".
+          inversion Heq; subst.
+          iSimpl.
+          iApply ewp_value.
+          apply of_to_val.
+          done.
+          iIntros (LI' HLI').
+          move/lfilledP in HLI'; inversion HLI'; subst.
+          inversion H8; subst.
+          iSimpl.
+          iApply ewp_br.
+          3:{ instantiate (1 := 0).
+              instantiate (1 := [AI_ref_cont kaddr]).
+              instantiate (1 := LH_base [] _).
+              rewrite /lfilled /lfill //=. } 
+          done.
+          done.
+          iApply ewp_value.
+          apply of_to_val.
+          done.
+          iRight. iRight.
+          iExists kaddr, h.
+          iSplit; first done.
+          iSplit; first done.
+          iCombine "Hb Hcont HI Hrunb" as "H".
+          iExact "H".
+        * iIntros (?) "[[[% _] | (% & % & % & % & _)] _]" => //.
+        * iIntros (??) "H".
+          iDestruct "H" as "[(%contb & -> & -> & Hcontb & Hrunb & HI & HQ1) | [(-> & -> & HQ1 & HQ2 & HI) | (%kaddr & %h & -> & -> & Hb & Hcont & HI & Hrunb)]]".
+          -- (* Case 1a *)
+            iApply ewp_value.
+            apply of_to_val.
+            done.
+            iIntros (LI HLI).
+            move/lfilledP in HLI; inversion HLI; subst.
+            inversion H8; subst.
+            iSimpl.
+            iApply ewp_br.
+            3:{
+              instantiate (1 := 1).
+              instantiate (1 := []).
+              instantiate (1 := LH_rec [] _ _ (LH_base [] _) _).
+              rewrite /lfilled /lfill //=. }
+            done.
+            done.
+(*            iNext. *)
+            iApply ("IH" $! kaddrb kaddrb 1).
+            iLeft.
+            iFrame "Hrunb".
+            iFrame.
+            by iRight.
+          -- (* Case 1b *)
+            iApply ewp_value.
+            apply of_to_val.
+            done.
+            iIntros (LI HLI).
+            move/lfilledP in HLI; inversion HLI; subst.
+            inversion H8; subst.
+            iSimpl.
+            iApply ewp_value.
+            apply of_to_val.
+            done.
+            iIntros (LI' HLI').
+            move/lfilledP in HLI'; inversion HLI'; subst.
+            inversion H11; subst.
+            iSimpl.
+            iApply ewp_br.
+            3:{
+              instantiate (1 := 2).
+              instantiate (1 := []).
+              instantiate (1 := LH_rec [] _ _ (LH_rec [] _ _ (LH_base [] _) _) _).
+              rewrite /lfilled /lfill //=. }
+            done.
+            done.
+(*            iNext. *)
+            iApply ewp_value.
+            apply of_to_val.
+            done.
+            iFrame.
+            done.
+          -- (* Case 2 *)
+            iSimpl.
+            rewrite (separate2 (AI_ref_cont _)).
+            iApply ewp_seq.
+            done.
+            iSplitR; last first.
+            iSplitR.
+            fold (AI_const (VAL_ref (VAL_ref_cont kaddr))).
+            iApply ewp_set_local.
+            simpl; lia.
+            iSimpl.
+            auto_instantiate.
+            2: by iIntros (?) "[% _]".
+            iIntros (??) "[-> ->]".
+            iSimpl.
+            rewrite (separate1 (AI_basic (BI_get_local _))).
+            iApply ewp_seq.
+            done.
+            iSplitR; last first.
+            iSplitR.
+            iApply ewp_get_local.
+            done.
+            auto_instantiate.
+            2: by iIntros (?) "[% _]".
+            iIntros (??) "[-> ->]".
+            iSimpl.
+            iDestruct "Hb" as "[(-> & %contb & Hconta & Hruna) | (-> & HQ2)]". 
+            ++ (* Case 2a: the other continuation is not done *)
+              rewrite (separate2 (AI_basic (BI_const _))).
+              iApply ewp_seq.
+              done.
+              iSplitR; last first.
+              iSplitR.
+              iApply ewp_br_if_false.
+              by subst.
+              auto_instantiate.
+              2: by iIntros (?) "[% _]".
+              iIntros (??) "[-> ->]".
+              iSimpl.
+              rewrite (separate1 (AI_basic (BI_get_local _))).
+              iApply ewp_seq.
+              done.
+              iSplitR; last first.
+              iSplitR.
+              iApply ewp_get_local.
+              done.
+              auto_instantiate.
+              2: by iIntros (?) "[% _]".
+              iIntros (??) "[-> ->]".
+              iSimpl.
+              rewrite (separate3 (AI_ref_cont _)).
+              iApply ewp_seq.
+              done.
+              iSplitR; last first.
+              iSplitR.
+              rewrite (separate1 (AI_ref_cont _)).
+              iApply ewp_val_app.
+              done.
+              iSplitR; last first.
+              rewrite (separate1 (AI_basic (BI_get_local 3))).
+              iApply ewp_wand_r. iSplitR.
+              iApply ewp_seq.
+              done.
+              iSplitR; last first.
+              iSplitR.
+              iApply ewp_get_local.
+              done.
+              auto_instantiate.
+              2: by iIntros (?) "[% _]".
+              iIntros (??) "[-> ->]".
+              iSimpl.
+              fold (AI_const (VAL_ref (VAL_ref_cont kaddrb))).
+              iApply ewp_set_local.
+              simpl; lia.
+              iSimpl.
+              auto_instantiate.
+              iIntros (??) "[-> ->]".
+              unfold val_combine. iSimpl.
+              auto_instantiate.
+              by iIntros "!>" (?) "[% _]".
+              2: by iIntros (?) "[% _]".
+              iIntros (??) "[->->]".
+              iSimpl.
+              rewrite (separate2 (AI_ref_cont _)).
+              iApply ewp_seq.
+              done.
+              iSplitR; last first.
+              iSplitR.
+              fold (AI_const (VAL_ref (VAL_ref_cont kaddr))).
+              iApply ewp_set_local.
+              simpl; lia.
+              iSimpl.
+              auto_instantiate.
+              2: by iIntros (?) "[% _]".
+              iIntros (??) "[-> ->]".
+              iSimpl.
+              iApply ewp_value.
+              apply of_to_val.
+              done.
+              iIntros (LI HLI).
+              move/lfilledP in HLI; inversion HLI; subst.
+              inversion H8; subst.
+              iSimpl.
+              iApply ewp_br.
+              3:{ instantiate (1 := 0).
+                  instantiate (1 := []).
+                  instantiate (1 := LH_base [] _).
+                  rewrite /lfilled /lfill //=. }
+              done. done.
+              iApply "IH".
+              iLeft.
+              iFrame "Hconta Hruna HI".
+              iLeft.
+              iSplit; first done.
+              iFrame "Hcont".
+              iNext.
+              iIntros "HI".
+              iDestruct ("Hrunb" with "HI") as "(%LI' & %HLI' & Hewp)".
+              iExists LI'.
+              iSplit; first by iPureIntro; destruct (hfilled No_var h [] LI').
+              iExact "Hewp".
+            ++ (* Case 2b: the other continuation is also done *)
+              rewrite (separate2 (AI_basic (BI_const _))).
+              iApply ewp_seq.
+              done.
+              iSplitR; last first.
+              iSplitR.
+              iApply ewp_br_if_true.
+              by subst.
+              iApply ewp_value.
+              apply of_to_val.
+              done.
+              iNext.
+              by instantiate (1 := λ v f, (⌜ v = brV _ ⌝ ∗ ⌜ f = Build_frame _ _ ⌝)%I).
+              2: by iIntros (?) "[% _]".
+              iIntros (??) "[-> ->]".
+              iSimpl.
+              iApply ewp_value.
+              apply of_to_val.
+              done.
+              iSimpl.
+              iIntros (LI HLI).
+              move/lfilledP in HLI; inversion HLI; subst.
+              inversion H8; subst.
+              iSimpl.
+              iApply ewp_br.
+              3:{ instantiate (1 := 0).
+                  instantiate (1 := []).
+                  instantiate (1 := LH_base [] _).
+                  rewrite /lfilled /lfill //=. }
+              done. done.
+              iApply "IH".
+              iRight.
+              iSplitL "HI"; first iExact "HI".
+              iFrame "Hcont".
+              iSplitL "Hrunb".
+              iIntros "!> HI".
+              iDestruct ("Hrunb" with "HI") as "(%LI' & %HLI' & Hewp)".
+              iExists LI'.
+              iSplit; first by iPureIntro; destruct (hfilled No_var h [] LI').
+              iExact "Hewp".
+              iRight.
+              iFrame. done.
+        * iIntros (?) "H".
+          iDestruct "H" as "[H | H]".
+          iDestruct "H" as (?) "[% _]" => //.
+          iDestruct "H" as "[H | H]".
+          iDestruct "H" as "[% _]" => //.
+          iDestruct "H" as (???) "[% _]" => //.
+  Qed. 
               
               
               
